src/salsa20/littleendian.lean
@@ -4,26 +4,52 @@
 -/
 import salsa20.words
 
+namespace littleendian
+
 -- Inputs and outputs:
 -- If b is a 4-byte sequence then littleendian(b) is a word.
 
--- If b = (b0, b1, b2, b3) then 
--- littleendian(b) = b0 + (2^8)*b1 + (2^16)*b2 + (2^24)*b3
+-- If b = (b₀, b₁, b₂, b₃) then 
+-- littleendian(b) = b₀ + (2^8)*b₁ + (2^16)*b₂ + (2^24)*b₃
 def littleendian (b : vector (bitvec byte_len) 4) : bitvec word_len := 
   bitvec.of_nat word_len (
-    (b.nth 0).to_nat + 
-    ((2^8) * (b.nth 1).to_nat) + 
-    ((2^16) * (b.nth 2).to_nat) + 
-    ((2^24) * (b.nth 3).to_nat))
+    (b.nth 0).to_nat +  ((2^8) * (b.nth 1).to_nat) + ((2^16) * (b.nth 2).to_nat) + ((2^24) * (b.nth 3).to_nat)
+  )
 
-#check littleendian
+lemma littleendian_zero :
+  (littleendian ([0, 0, 0, 0].to_vec_of_bitvec byte_len 4)).to_nat = 0 := rfl
 
+-- The inverse of little-endian is indeed the function that sends a word (32 bits) 
+-- back to the sequence of 4 bytes in a little endian way, so the least significant
+-- byte goes first, and the most significant byte goes last. 
+-- So it maps 𝑤 to w & 0xff, (w >> 8) & 0xff, (w >> 16) & 0xff, (w >> 24) & 0xff
+--
+-- https://crypto.stackexchange.com/a/22314
+def littleendian_inv (w : bitvec word_len) : vector (bitvec byte_len) 4 :=
+  [
+    bitvec.of_nat byte_len (bitvec.to_nat((bitvec.and w 0xff))),
+    bitvec.of_nat byte_len (bitvec.to_nat(((bitvec.ushr w 8).and 0xff))),
+    bitvec.of_nat byte_len (bitvec.to_nat(((bitvec.ushr w 16).and 0xff))), 
+    bitvec.of_nat byte_len (bitvec.to_nat(((bitvec.ushr w 24).and 0xff)))
+  ].to_vec_of_bitvec byte_len 4
+
+lemma littleendian_inv_zero :
+  littleendian_inv 0 = ([0, 0, 0, 0].to_vec_of_bitvec byte_len 4) := rfl
+
+
+lemma inv_undoes_littleendian (b0 b1 b2 b3 : bitvec byte_len) : 
+  (littleendian_inv (littleendian ([b0, b1, b2, b3].to_vec_of_bitvec byte_len 4))).to_list = 
+    [b0, b1, b2, b3] :=
+begin
+  sorry,
+end
+
+
+namespace examples
+
+-- littleendian
 #eval (littleendian ([0, 0, 0, 0].to_vec_of_bitvec byte_len 4)).to_nat
 #eval 0x00000000
-
-lemma littleendian_zero : 
-  (littleendian ([0, 0, 0, 0].to_vec_of_bitvec byte_len 4)).to_nat = 0 
-  := rfl
 
 #eval bitvec.to_nat (littleendian ([86, 75, 30, 9].to_vec_of_bitvec byte_len 4))
 #eval 0x091e4b56
@@ -34,14 +60,7 @@ lemma littleendian_zero :
 #eval bitvec.to_nat (littleendian ([255, 255, 255, 255].to_vec_of_bitvec byte_len 4))
 #eval 0xffffffff
 
--- https://crypto.stackexchange.com/a/22314
-def littleendian_inv (w : bitvec word_len) : vector (bitvec byte_len) 4 :=
-  [
-    bitvec.of_nat byte_len (bitvec.to_nat((bitvec.and w 0xff))),
-    bitvec.of_nat byte_len (bitvec.to_nat(((bitvec.ushr w 8).and 0xff))),
-    bitvec.of_nat byte_len (bitvec.to_nat(((bitvec.ushr w 16).and 0xff))), 
-    bitvec.of_nat byte_len (bitvec.to_nat(((bitvec.ushr w 24).and 0xff)))
-  ].to_vec_of_bitvec byte_len 4
+-- littleendian_inv
 
 #eval (littleendian_inv 0x00000000).to_list
 
@@ -54,9 +73,7 @@ def littleendian_inv (w : bitvec word_len) : vector (bitvec byte_len) 4 :=
 
 #eval (littleendian_inv 0xfaffffff).to_list
 
-lemma inv_undoes_littleendian (b0 b1 b2 b3 : bitvec byte_len) : 
-  (littleendian_inv (littleendian ([b0, b1, b2, b3].to_vec_of_bitvec byte_len 4))).to_list = 
-    [b0, b1, b2, b3] :=
-begin
-  sorry,
-end
+
+end examples
+
+end littleendian
